Fix instance locality

theories/Symbolic/Instantiation.v
@@ -65,35 +65,35 @@ Module Type InstantiationOn
     inst : forall {Σ}, T Σ -> Valuation Σ -> A.
   Class Lift (T : LCtx -> Type) (A : Type) : Type :=
     lift : forall {Σ}, A -> T Σ.
+  #[global] Arguments inst {T A _ Σ} !_ ι.
+  #[global] Arguments lift {T A _ Σ} !_.
 
-  Instance inst_list {T : LCtx -> Type} {A : Type} `{Inst T A} :
+  #[export] Instance inst_list {T : LCtx -> Type} {A : Type} `{Inst T A} :
     Inst (List T) (list A) := fun Σ xs ι => List.map (fun x => inst x ι) xs.
-  Instance lift_list {T : LCtx -> Type} {A : Type} `{Lift T A} :
+  #[export] Instance lift_list {T : LCtx -> Type} {A : Type} `{Lift T A} :
     Lift (List T) (list A) := fun Σ => List.map lift.
 
-  Instance inst_const {A} `{finite.Finite A} :
+  #[export] Instance inst_const {A} `{finite.Finite A} :
     Inst (Const A) A := fun Σ x ι => x.
-  Instance lift_const {A} `{finite.Finite A} :
+  #[export] Instance lift_const {A} `{finite.Finite A} :
     Lift (Const A) A := fun Σ x => x.
 
-  Instance inst_env {T : Set} {S : LCtx -> T -> Set}
-         {A : T -> Set} {InstSA : forall τ : T, Inst (fun Σ => S Σ τ) (A τ)}
-         {Γ : Ctx T} :
+  #[export] Instance inst_env {T : Set} {S : LCtx -> T -> Set} {A : T -> Set}
+    {InstSA : forall τ : T, Inst (fun Σ => S Σ τ) (A τ)} {Γ : Ctx T} :
     Inst (fun Σ => Env (S Σ) Γ) (Env A Γ) :=
     fun Σ xs ι => env.map (fun (b : T) (s : S Σ b) => inst s ι) xs.
-  Instance lift_env {T : Set} {S : LCtx -> T -> Set}
-         {A : T -> Set} {InstSA : forall τ : T, Lift (fun Σ => S Σ τ) (A τ)}
-         {Γ : Ctx T} :
+  #[export] Instance lift_env {T : Set} {S : LCtx -> T -> Set} {A : T -> Set}
+    {InstSA : forall τ : T, Lift (fun Σ => S Σ τ) (A τ)} {Γ : Ctx T} :
     Lift (fun Σ => Env (S Σ) Γ) (Env A Γ) :=
     fun Σ => env.map (fun (b : T) (a : A b) => lift a).
 
   Lemma inst_env_snoc {B : Set} {AT : LCtx -> B -> Set}
-         {A : B -> Set} {_ : forall b : B, Inst (fun Σ => AT Σ b) (A b)}
-         {Γ : Ctx B} {Σ} (ι : Valuation Σ) (E : Env (AT Σ) Γ) (b : B) (a : AT Σ b) :
+    {A : B -> Set} {_ : forall b : B, Inst (fun Σ => AT Σ b) (A b)}
+    {Γ : Ctx B} {Σ} (ι : Valuation Σ) (E : Env (AT Σ) Γ) (b : B) (a : AT Σ b) :
     inst (env.snoc E b a) ι = env.snoc (inst E ι) b (inst a ι).
   Proof. reflexivity. Qed.
 
-  Instance inst_term : forall {σ}, Inst (fun Σ => Term Σ σ) (Val σ) :=
+  #[export] Instance inst_term : forall {σ}, Inst (fun Σ => Term Σ σ) (Val σ) :=
     fix inst_term {σ : Ty} {Σ : LCtx} (t : Term Σ σ) (ι : Valuation Σ) {struct t} : Val σ :=
     match t in Term _ σ return Val σ with
     | @term_var _ _ _ bIn  => env.lookup ι bIn
@@ -108,10 +108,10 @@ Module Type InstantiationOn
         let InstTerm xt := @inst_term (@type recordf Ty xt) in
         recordv_fold R (inst (Inst := inst_env (InstSA := InstTerm)) ts ι)
     end.
-  Instance lift_term {σ} : Lift (fun Σ => Term Σ σ) (Val σ) :=
+  #[export] Instance lift_term {σ} : Lift (fun Σ => Term Σ σ) (Val σ) :=
     fun Σ v => term_val σ v.
 
-  Instance inst_sub {Σ} : Inst (Sub Σ) (Valuation Σ) :=
+  #[export] Instance inst_sub {Σ} : Inst (Sub Σ) (Valuation Σ) :=
     inst_env.
 
   Class InstSubst (T : LCtx -> Type) (A : Type) `{Inst T A, Subst T} : Prop :=
@@ -124,7 +124,7 @@ Module Type InstantiationOn
   Arguments InstSubst T A {_ _}.
   Arguments InstLift T A {_ _}.
 
-  Instance inst_subst_list {T : LCtx -> Set} {A : Set} `{InstSubst T A} :
+  #[export] Instance inst_subst_list {T : LCtx -> Set} {A : Set} `{InstSubst T A} :
     InstSubst (List T) (list A).
   Proof.
     intros ? ? ζ ι xs.
@@ -134,7 +134,7 @@ Module Type InstantiationOn
     apply List.map_ext, inst_subst.
   Qed.
 
-  Instance inst_lift_list {T : LCtx -> Set} {A : Set} `{InstLift T A} :
+  #[export] Instance inst_lift_list {T : LCtx -> Set} {A : Set} `{InstLift T A} :
     InstLift (List T) (list A).
   Proof.
     intros Σ ι a. unfold inst, inst_list, lift, lift_list.
@@ -142,15 +142,15 @@ Module Type InstantiationOn
     apply List.map_ext, inst_lift.
   Qed.
 
-  Instance inst_subst_const {A} `{finite.Finite A} :
+  #[export] Instance inst_subst_const {A} `{finite.Finite A} :
     InstSubst (Const A) A.
   Proof. intros ? ? ζ ι t. reflexivity. Qed.
 
-  Instance inst_lift_const {A} `{finite.Finite A} :
+  #[export] Instance inst_lift_const {A} `{finite.Finite A} :
     InstLift (Const A) A.
   Proof. intros ? ι a. reflexivity. Qed.
 
-  Instance inst_subst_env {T : Set} {S : LCtx -> T -> Set} {A : T -> Set}
+  #[export] Instance inst_subst_env {T : Set} {S : LCtx -> T -> Set} {A : T -> Set}
          {_ : forall τ : T, Inst (fun Σ => S Σ τ) (A τ)}
          {_ : forall τ : T, Subst (fun Σ => S Σ τ)}
          {_ : forall τ : T, InstSubst (fun Σ => S Σ τ) (A τ)}
@@ -163,7 +163,7 @@ Module Type InstantiationOn
     intros b s; apply inst_subst.
   Qed.
 
-  Instance inst_lift_env {T : Set} {S : LCtx -> T -> Set} {A : T -> Set}
+  #[export] Instance inst_lift_env {T : Set} {S : LCtx -> T -> Set} {A : T -> Set}
          {_ : forall τ : T, Inst (fun Σ => S Σ τ) (A τ)}
          {_ : forall τ : T, Lift (fun Σ => S Σ τ) (A τ)}
          {_ : forall τ : T, InstLift (fun Σ => S Σ τ) (A τ)}
@@ -176,7 +176,7 @@ Module Type InstantiationOn
     intros; apply inst_lift.
   Qed.
 
-  Instance inst_subst_term {σ} : InstSubst (fun Σ => Term Σ σ) (Val σ).
+  #[export] Instance inst_subst_term {σ} : InstSubst (fun Σ => Term Σ σ) (Val σ).
   Proof.
     unfold InstSubst.
     induction t; cbn; try (repeat f_equal; auto; fail).
@@ -185,13 +185,13 @@ Module Type InstantiationOn
     - f_equal. induction IH; cbn; now f_equal.
   Qed.
 
-  Instance inst_lift_term {σ} : InstLift (fun Σ => Term Σ σ) (Val σ).
+  #[export] Instance inst_lift_term {σ} : InstLift (fun Σ => Term Σ σ) (Val σ).
   Proof. red. reflexivity. Qed.
 
-  Instance inst_subst_sub {Σ} : InstSubst (Sub Σ) (Valuation Σ).
+  #[export] Instance inst_subst_sub {Σ} : InstSubst (Sub Σ) (Valuation Σ).
   Proof. apply inst_subst_env. Qed.
 
-  Instance inst_lift_sub {Σ} : InstLift (Sub Σ) (Valuation Σ).
+  #[export] Instance inst_lift_sub {Σ} : InstLift (Sub Σ) (Valuation Σ).
   Proof. apply inst_lift_env. Qed.
 
   Lemma inst_sub_wk1 {Σ b v} (ι : Valuation Σ) :
@@ -327,51 +327,48 @@ Module Type InstantiationOn
       f_equal. now eapply IHσs.
   Qed.
 
-  Global Arguments inst {T A _ Σ} !_ ι.
-  Global Arguments lift {T A _ Σ} !_.
-
-  Instance inst_unit : Inst Unit unit :=
+  #[export] Instance inst_unit : Inst Unit unit :=
     fun _ x ι => x.
-  Instance lift_unit : Lift Unit unit :=
+  #[export] Instance lift_unit : Lift Unit unit :=
     fun _ x => x.
 
-  Instance inst_subst_unit : InstSubst Unit unit.
+  #[export] Instance inst_subst_unit : InstSubst Unit unit.
   Proof. red. reflexivity. Qed.
-  Instance inst_lift_unit : InstLift Unit unit.
+  #[export] Instance inst_lift_unit : InstLift Unit unit.
   Proof. red. reflexivity. Qed.
 
-  Instance inst_pair {AT BT A B} `{Inst AT A, Inst BT B} :
+  #[export] Instance inst_pair {AT BT A B} `{Inst AT A, Inst BT B} :
     Inst (Pair AT BT) (A * B) :=
     fun Σ '(a , b) ι => (inst a ι, inst b ι).
-  Instance lift_pair {AT BT A B} `{Lift AT A, Lift BT B} :
+  #[export] Instance lift_pair {AT BT A B} `{Lift AT A, Lift BT B} :
     Lift (Pair AT BT) (A * B) :=
     fun Σ '(a, b) => (lift a , lift b).
 
-  Instance inst_subst_pair {AT BT A B} `{InstSubst AT A, InstSubst BT B} :
+  #[export] Instance inst_subst_pair {AT BT A B} `{InstSubst AT A, InstSubst BT B} :
     InstSubst (Pair AT BT) (A * B).
   Proof. intros ? ? ? ? []; cbn; f_equal; apply inst_subst. Qed.
 
-  Instance inst_lift_pair {AT BT A B} `{InstLift AT A, InstLift BT B} :
+  #[export] Instance inst_lift_pair {AT BT A B} `{InstLift AT A, InstLift BT B} :
     InstLift (Pair AT BT) (A * B).
   Proof. intros ? ? []; cbn; f_equal; apply inst_lift. Qed.
 
-  Instance inst_option {AT A} `{Inst AT A} : Inst (Option AT) (option A) :=
+  #[export] Instance inst_option {AT A} `{Inst AT A} : Inst (Option AT) (option A) :=
     fun Σ ma ι => option_map (fun a => inst a ι) ma.
-  Instance lift_option {AT A} `{Lift AT A} : Lift (Option AT) (option A) :=
+  #[export] Instance lift_option {AT A} `{Lift AT A} : Lift (Option AT) (option A) :=
     fun Σ ma => option_map lift ma.
 
-  Instance inst_subst_option {AT A} `{InstSubst AT A} :
+  #[export] Instance inst_subst_option {AT A} `{InstSubst AT A} :
     InstSubst (Option AT) (option A).
   Proof. intros ? ? ? ? []; cbn; f_equal; apply inst_subst. Qed.
-  Instance inst_lift_option {AT A} `{InstLift AT A} :
+  #[export] Instance inst_lift_option {AT A} `{InstLift AT A} :
     InstLift (Option AT) (option A).
   Proof. intros ? ? []; cbn; f_equal; apply inst_lift. Qed.
 
-  Instance inst_store {Γ} : Inst (SStore Γ) (CStore Γ) :=
+  #[export] Instance inst_store {Γ} : Inst (SStore Γ) (CStore Γ) :=
     inst_env.
-  Instance inst_subst_store {Γ} : InstSubst (SStore Γ) (CStore Γ).
+  #[export] Instance inst_subst_store {Γ} : InstSubst (SStore Γ) (CStore Γ).
   Proof. apply inst_subst_env. Qed.
-  Instance inst_lift_store {Γ} : InstLift (SStore Γ) (CStore Γ).
+  #[export] Instance inst_lift_store {Γ} : InstLift (SStore Γ) (CStore Γ).
   Proof. apply inst_lift_env. Qed.
 
   Section Utils.
