theories/Syntax/Predicates.v
@@ -48,7 +48,7 @@ Module Type PurePredicateKit (Import B : Base).
   Parameter Inline 𝑷_Ty : 𝑷 -> Ctx Ty.
   Parameter Inline 𝑷_inst : forall p : 𝑷, env.abstract Val (𝑷_Ty p) Prop.
 
-  Declare Instance 𝑷_eq_dec : EqDec 𝑷.
+  #[export] Declare Instance 𝑷_eq_dec : EqDec 𝑷.
 
 End PurePredicateKit.
 
@@ -59,9 +59,9 @@ Module Type HeapPredicateKit (Import B : Base).
   (* Predicate field types. *)
   Parameter Inline 𝑯_Ty : 𝑯 -> Ctx Ty.
   (* Duplicable? *)
-  Declare Instance 𝑯_is_dup : IsDuplicable 𝑯.
+  #[export] Declare Instance 𝑯_is_dup : IsDuplicable 𝑯.
 
-  Declare Instance 𝑯_eq_dec : EqDec 𝑯.
+  #[export] Declare Instance 𝑯_eq_dec : EqDec 𝑯.
 
   Parameter 𝑯_precise : forall p : 𝑯, option (Precise 𝑯_Ty p).
 
@@ -75,7 +75,7 @@ Module DefaultPurePredicateKit (Import B : Base) <: PurePredicateKit B.
   Definition 𝑷 := Empty_set.
   Definition 𝑷_Ty : 𝑷 -> Ctx Ty := fun p => match p with end.
   Definition 𝑷_inst (p : 𝑷) : env.abstract Val (𝑷_Ty p) Prop := match p with end.
-  Instance 𝑷_eq_dec : EqDec 𝑷 := fun p => match p with end.
+  #[export] Instance 𝑷_eq_dec : EqDec 𝑷 := fun p => match p with end.
 
 End DefaultPurePredicateKit.
 
@@ -83,8 +83,8 @@ Module DefaultHeapPredicateKit (Import B : Base) <: HeapPredicateKit B.
 
   Definition 𝑯 := Empty_set.
   Definition 𝑯_Ty : 𝑯 -> Ctx Ty := fun p => match p with end.
-  Instance 𝑯_eq_dec : EqDec 𝑯 := fun p => match p with end.
-  Instance 𝑯_is_dup : IsDuplicable 𝑯 := { is_duplicable := fun p => match p with end }.
+  #[export] Instance 𝑯_eq_dec : EqDec 𝑯 := fun p => match p with end.
+  #[export] Instance 𝑯_is_dup : IsDuplicable 𝑯 := { is_duplicable := fun p => match p with end }.
   Definition 𝑯_precise (p : 𝑯) : option (Precise 𝑯_Ty p) := None.
 
 End DefaultHeapPredicateKit.
